selsort: proof.

sorting-algorithms/SelectionSort.v
@@ -7,13 +7,46 @@ Require Import SortSpec.
 Require Import Tactics.Bool2Prop.
 Require Import Tactics.CpdtTactics.
 
-(** Formalizing and proving selection sort based on dependent type. *)
+(** Formalizing and proving selection sort based on dependent type
+    and generic recursion. *)
 
 (** The original idea is presented by Andrew Appel in OPLSS14, but his
     implementation was a little hacky, the [selsort_aux] function only
     takes two parameters [l] and [n], but uses the assumption that
     [length l] = [n]. So I enhance his implementation using dependent
-    type, where we encode the proof of the equality in program. *)
+    type and generic recursion, where we "encode" the proof of the
+    equality in program. *)
+
+(* The proof outline is very similar to quicksort. *)
+
+Lemma Forall_Permutation :
+  forall A (l l' : list A) P, Forall P l -> Permutation l l' -> Forall P l'.
+Proof.
+  intros. apply Forall_forall.
+  intros. apply Permutation_sym in H0.
+  eapply Permutation_in in H0; eauto.
+  rewrite Forall_forall in H.
+  apply H. apply H0.
+Qed.
+
+Definition AllLe (x : nat) (l : list nat) : Prop := Forall (fun y => x <= y) l.
+
+Definition lengthOrder (l1 l2 : list nat) :=
+  length l1 < length l2.
+
+Lemma lengthOrder_wf' :
+  forall len l, length l <= len -> Acc lengthOrder l.
+Proof.
+  Hint Constructors Acc.
+  unfold lengthOrder; induction len; crush.
+Defined.
+
+(** [lengthOrder] is well-founded relation. *)
+Theorem lengthOrder_wf : well_founded lengthOrder.
+Proof.
+  Hint Constructors Acc.
+  unfold lengthOrder; intro; eapply lengthOrder_wf'; eauto.
+Defined.
 
 Fixpoint select (i : nat) (l : list nat) : nat * list nat :=
   match l with
@@ -23,34 +56,70 @@ Fixpoint select (i : nat) (l : list nat) : nat * list nat :=
                 else let (j, l') := select h t in (j, i :: l')
   end.
 
+Lemma select_spec :
+  forall l x h t,
+    select x l = (h, t) -> AllLe h (x :: l) /\ Permutation (x :: l) (h :: t).
+Proof.
+  intro l; induction l; crush.
+  - constructor; auto.
+  - destruct (x <? a) eqn:Heq; b2p; crush.
+    destruct (select x l) eqn:Hs; apply IHl in Hs; inversion H; crush.
+    inversion H0; subst; repeat constructor; crush.
+    destruct (select a l) eqn:Hs; apply IHl in Hs; inversion H; crush.
+    inversion H0; subst; repeat constructor; crush.
+  - destruct (x <? a) eqn:Heq; b2p; crush.
+    destruct (select x l) eqn:Hs; apply IHl in Hs; inversion H; crush.
+    eapply perm_trans. apply perm_swap. eapply perm_trans.
+    apply perm_skip. apply H3. apply perm_swap.
+    destruct (select a l) eqn:Hs; apply IHl in Hs; inversion H; crush.
+    apply perm_swap.
+Qed.
+
+Lemma select_spec' :
+  forall l x h t,
+    select x l = (h, t) -> AllLe h t /\ Permutation (x :: l) (h :: t).
+Proof.
+  intros; pose proof (select_spec l x h t H); crush.
+  unfold AllLe in *.
+  assert (Forall (fun y : nat => h <= y) (h :: t)).
+  { eapply Forall_Permutation; eauto. }
+  inversion H0; auto.
+Qed.
+
 Lemma select_len :
   forall l x h t,
     select x l = (h, t) -> length t = length l.
 Proof.
-  intro l; induction l; crush; destruct (x <? a); crush.
-  destruct (select x l) eqn:Heq; crush; pose proof (IHl x h l0) Heq; crush.
-  destruct (select a l) eqn:Heq; crush; pose proof (IHl a h l0) Heq; crush.
+  intros; pose proof (select_spec l x h t H); crush.
+  apply Permutation_length in H2; crush.
 Qed.
 
 (* Use the idea of "convey pattern" mentioned by Adam Chlipala in
    http://coq-club.inria.narkive.com/Jz4riTaq/equations-from-match-case-unifiers-under-refine-tactic *)
-Fixpoint selsort_aux (l : list nat) (n : nat) (H : length l = n) : list nat.
-  refine (
-    match l, n return length l = n -> list nat with
-    | h :: t, S n' =>
-        fun H => match select h t as p return length (snd p) = n' -> list nat with
-                 | (x, l') => fun H => x :: selsort_aux l' n' H
-                 end _
-    | nil, 0 =>
-        fun H => nil
-    | _, _ => _
-    end H
-  ); crush. destruct (select h t) eqn:Heq; simpl; eapply select_len; eauto.
+Definition selsort : list nat -> list nat.
+  refine (Fix lengthOrder_wf (fun _ => list nat)
+    (fun (l : list nat) =>
+      match l return (forall l' : list nat, lengthOrder l' l -> list nat) -> list nat with
+      | nil => fun H => nil
+      | h :: t =>
+          fun (selsort : forall l' : list nat, lengthOrder l' (h :: t) -> list nat) =>
+            fst (select h t) :: selsort (snd (select h t)) _
+      end
+	  )
+	); unfold lengthOrder; destruct (select h t) eqn:H; pose proof (select_len t h n l0 H); crush.
 Defined.
 
-Definition selsort (l : list nat) : list nat.
-  refine (selsort_aux l (length l) _); reflexivity.
-Defined.
+Theorem selsort_eq : forall l,
+  selsort l =
+    match l with
+    | nil => nil
+    | h :: t => fst (select h t) :: selsort (snd (select h t))
+    end.
+Proof.
+  intros; destruct l; auto.
+  apply (Fix_eq lengthOrder_wf (fun _ => list nat)). intros.
+  destruct x; simpl; repeat f_equal; auto.
+Qed.
 
 Notation "[ ]" := nil.
 Notation "[ x , .. , y ]" := (cons x .. (cons y nil) ..).
@@ -58,4 +127,23 @@ Example selsort_pi :
   selsort [3, 1, 4, 1, 5, 9, 2, 6, 5, 3, 5] = [1, 1, 2, 3, 3, 4, 5, 5, 5, 6, 9].
 Proof.
   simpl; reflexivity.
+Qed.
+
+Theorem selsort_ok :
+  SortSpec selsort.
+Proof.
+  unfold selsort, SortSpec.
+  intros.
+  apply (well_founded_ind lengthOrder_wf
+    (fun l => Sorted (selsort l) /\ Permutation l (selsort l))
+  ).
+  intros; rewrite selsort_eq; destruct x; auto.
+  destruct (select n x) eqn:Heq; simpl.
+  pose proof (select_len x n n0 l0 Heq).
+  assert (Hl: lengthOrder l0 (n :: x)). { unfold lengthOrder; crush. }
+  pose proof (H l0 Hl).
+  apply select_spec' in Heq; crush.
+  assert (AllLe n0 (selsort l0)). { eapply Forall_Permutation; eauto. }
+  destruct (selsort l0); auto.
+  constructor; inversion H1; crush.
 Qed.
